Phi_Semantics/PhiSem_Generic_Boolean.thy
@@ -1,7 +1,7 @@
 chapter \<open>Generic Boolean\<close>
 
 theory PhiSem_Generic_Boolean
-  imports Phi_System.PhiSem_Formalization_Tools
+  imports Phi_System.PhiSem_Formalization_Tools2
 begin
 
 section \<open>Semantics\<close>
